HybridVerifVecs/rels/kat2rel.thy
@@ -115,24 +115,7 @@ lemma sH_g_evolution_inv:
   using assms(2) by simp
 
 lemma sH_diff_inv: "rel_kat.H \<lceil>I\<rceil> (x\<acute>=f & G on T S @ t\<^sub>0) \<lceil>I\<rceil> = diff_invariant I f T S t\<^sub>0 G"
-  unfolding diff_invariant_eq sH_H g_orbital_eq by auto
-
-context local_flow
-begin
-
-lemma wp_diff_inv_eq:
-  assumes "S = UNIV"
-  shows "(rel_kat.H  \<lceil>I\<rceil> (x\<acute>=f & (\<lambda>s. True) on T S @ 0) \<lceil>I\<rceil>) = diff_invariant I f T S 0 (\<lambda>s. True)"
-  unfolding diff_invariant_eq[OF assms] sH_H using g_orbital_collapses unfolding assms 
-  by clarsimp force
-
-lemma wp_orbit_inv_eq:
-  assumes "S = UNIV"
-  shows "(rel_kat.H  \<lceil>I\<rceil>  ({(s,s') | s s'. s' \<in> \<gamma>\<^sup>\<phi> s}) \<lceil>I\<rceil>) = (\<forall>s\<in>S. \<forall>t\<in>T. I s \<longrightarrow> I (\<phi> t s))"
-  unfolding orbit_def wp_diff_inv_eq[OF assms] diff_invariant_eq[OF assms] 
-  using in_ivp_sols ivp(2) init_time unfolding assms by auto
-
-end
+  unfolding diff_invariant_eq sH_H g_orbital_eq image_le_pred by auto
 
 subsection\<open> Derivation of the rules of dL \<close>
 
